incr/IncrAll.v
@@ -1,11 +1,10 @@
-(* Require Import CRIS Cancel.
+Require Import CRIS Cancel.
 Require Import MemI MemA MemIAproof ImpPrelude.
-From CRIS.incr Require Import Header ClientI ClientA ClientIA FaaI FaaA FaaIA.
 Require Import SchHeader SchI SchA SchIAproof SchTactics.
+From CRIS.incr Require Import Header ClientI ClientA ClientIA FaaI FaaA FaaIA.
 
 Module ClientAll.
   Import inv_instances.
-  (* Local Definition u : univ_id := 1. *)
 
   Local Definition csl : string → bool := λ _, false.
   Local Definition genv : GEnv.t := GEnv.unit.
@@ -27,44 +26,62 @@ Module ClientAll.
   Qed.
 
   (* source module *)
-  Local Definition sp_user_s : string → option fspec :=
-    to_sp (ClientA.sp ⊤ ++ MemA.sp).
+  Local Definition sp_user_s : spl_type :=
+    ClientA.sp ⊤ 1%Qp.
   Local Definition smod_src : SMod.t :=
-    (ClientA.Mod ⊤) ☆ (MemA.Mod) ☆ (SchA.Mod ⊤ sp_user_s ☆ SchAPure.Mod ⊤).
-  Local Definition sp_s : string → option fspec := sp_from smod_src.
+    (ClientA.smod ⊤ 1%Qp) ☆ (SchA.smod sp_user_s).
+  Local Definition sp : string → option fspec := sp_from smod_src.
 
-  Local Definition smod_cancel : Mod.t := SModCancel.to_mod smod_src.
-  Local Definition mod_src : Mod.t := SMod.to_mod sp_s smod_src.
+  Local Definition mod_top : Mod.t := SMod.to_mod sp_none (SMod.cancel smod_src).
+  Local Definition mod_src : Mod.t := SMod.to_mod sp smod_src.
   Local Definition mod_tgt : Mod.t := ClientI.t ★ FaaI.t ★ (MemI.t csl genv) ★ (SchI.t).
 
-  Local Definition SchInSp0: sp_incl (SchAS.sp ⊤ (to_sp [])) (to_sp (SchAS.sp ⊤ (to_sp []))).
+  (* Local Definition SchInSp0: sp_incl (SchAS.sp ⊤ (to_sp [])) (to_sp (SchAS.sp ⊤ (to_sp []))).
   Proof.
     split; [|refl]. rewrite /SchAS.sp; unseal CRIS. prove_nodup.
-  Qed.
-  Local Definition SchInSp : sp_incl (SchAS.sp ⊤ sp_user_s) sp_s.
+  Qed. *)
+  Local Definition SchInSp : sp_incl (SchAS.sp sp_user_s ⊤ 1%Qp) sp.
   Proof.
-    ii; rewrite /sp_s /SchAS.sp /MemA.sp /ClientA.sp; unseal CRIS; split; [prove_nodup|ii].
-    ss; des_ifs; rewrite ->eq_rel_dec_correct in *; des_ifs.
+    rewrite /SchAS.sp; unseal CRIS.
+    split; [prove_nodup|].
+    intros ??; ss; des_ifs; des_sumbool; clarify; intros INV; inv INV;
+      rewrite /sp /smod_src /sp_from /= /to_sp /=; des_ifs; ss.
   Qed.
-  Local Definition MainInSp : sp_incl (ClientA.sp ⊤) sp_user_s.
+  Local Definition UserInSp : sp_incl sp_user_s sp.
   Proof.
-    ii; rewrite /sp_s /SchAS.sp /MemA.sp /ClientA.sp; unseal CRIS; split; [prove_nodup|ii].
-    ss; des_ifs; rewrite ->eq_rel_dec_correct in *; des_ifs.
+    rewrite /sp_user_s /ClientA.sp /MemA.sp; unseal CRIS.
+    split; [prove_nodup|].
+    intros ??; ss; des_ifs; des_sumbool; clarify; intros INV; inv INV;
+      rewrite /sp /smod_src /sp_from /= /to_sp /=; des_ifs; ss.
   Qed.
-  Local Definition MemInSp : sp_incl MemA.sp sp_s.
+  Local Definition MainInSp : spl_sub (ClientA.sp ⊤ 1%Qp) sp_user_s.
   Proof.
-    ii; rewrite /sp_s /SchAS.sp /MemA.sp /ClientA.sp; unseal CRIS; split; [prove_nodup|ii].
-    ss; des_ifs; rewrite ->eq_rel_dec_correct in *; des_ifs.
+    rewrite /spl_sub /sp_user_s /ClientA.sp /ClientA.incr_spec /=.
+    ii; rewrite ->eq_rel_dec_correct in *; des_ifs.
   Qed.
+  (* Local Definition MemInSp : sp_incl MemA.sp sp.
+  Proof.
+    ii; rewrite /sp /SchAS.sp /MemA.sp /ClientA.sp; unseal CRIS; split; [prove_nodup|ii].
+    ss; des_ifs; rewrite ->eq_rel_dec_correct in *; des_ifs.
+  Qed. *)
 
-  Local Definition init_cond : iProp Σ := MemA.init_cond csl genv ∗ SchA.init_cond.
-  Local Definition main_fsp : fspec := ClientA.main_spec ⊤.
+  Local Definition init_cond : iProp Σ :=
+    MemA.init_cond csl genv ∗ SchA.init_cond ∗ ClientIA.ClientIA.init_cond ⊤ 1%Qp.
+  (* Local Definition main_fsp : fspec := ClientA.main_spec ⊤ 1%Qp. *)
 
   (* Apply cancellation to linked spec module *)
   Lemma cancel_src :
-    refines (smod_cancel, (init_cond ∗ main_fsp.(precond) (0, tt) tt↑ tt↑)%I) 
-            (mod_src, init_cond).
-  Proof. i; eapply cancellation; try by econs. i. iIntros "[_ [_ %POST]]". iPureIntro. des; eauto. Qed.
+    refines (mod_top, init_cond) (mod_src, init_cond).
+  Proof.
+    eapply Cancel.cancellation.
+    { ii; des; subst; inv FIND; ss.
+      rewrite !eq_rel_dec_correct in H0; des_ifs.
+    }
+    { econs; [refl|]; i; inv NS; des; inv H; des; inv H1;
+      rewrite !eq_rel_dec_correct in H2; des_ifs.
+    }
+    { econs; unfold_mod; ss; prove_nodup. }
+  Qed.
 
   (* Refinement between spec/impl of whole program (linked module) *)
   Lemma src_tgt : refines (mod_src, init_cond) (mod_tgt, emp%I).
@@ -77,8 +94,7 @@ Module ClientAll.
     { do 3 ctxr_drop.
       eapply main_adequacy, SchIA.sim.
       - apply SchInSp.
-      - rewrite /sp_sub /sp_user_s /sp_s /ClientA.sp /MemA.sp; unseal CRIS.
-        ii; ss. des_ifs; rewrite ->eq_rel_dec_correct in *; des_ifs.
+      - apply UserInSp.
     }
 
     (* abstraction of Mem *)
@@ -91,7 +107,6 @@ Module ClientAll.
     etrans; cycle 1.
     { do 2 ctxr_drop.
       eapply main_adequacy, FaaIA.sim.
-      (* apply SchInSp0. *)
     }
     rewrite /FaaIA.FaaIA.MA.
     
@@ -102,25 +117,27 @@ Module ClientAll.
       - instantiate (1:=⊤). set_solver.
       - apply MainInSp.
       - apply SchInSp.
-      (* - apply SchInSp0.
-      - apply MemInSp.
-      - unfold u. nia. *)
     }
 
     etrans; cycle 1.
     { ctxr_rotate. ctxr_refl. }
-    
+
+    (* elimination of mem *)
+    etrans; cycle 1.
+    { do 2 ctxr_rotate. do 2 ctxr_drop. eapply CFilter.elim_module. }
+    rewrite -mod_add_empty_r.
+
     rewrite /SchIAproof.SchIA.SchAMod.
-    rewrite /SchIAproof.SchIA.SchA /SchIAproof.SchIA.SchAPure.
-    rewrite /SchA.t /SchAPure.t /ClientA.t /MemA.t.
+    rewrite /SchA.t /ClientA.t /MemA.t.
     unseal CRIS.
+    ctxr_rotate.
     
     eapply ctxr_cond_strengthen.
-    { iIntros "[? ?]". iFrame. }
+    { iIntros "[? [? ?]]". iFrame. }
   (*SLOW*)Admitted.
 
   Lemma cancel_tgt :
-    refines (smod_cancel, (init_cond ∗ main_fsp.(precond) (0, tt) tt↑ tt↑)%I)
+    refines (mod_top, init_cond)
             (mod_tgt, emp%I).
   Proof.
     etrans.
@@ -129,9 +146,9 @@ Module ClientAll.
   Qed.
 
   Theorem behavioral_refinement :
-    ∃ target_resource, refines_mod
-      (Mod.to_mod smod_cancel (IRΣ ⋅ ir_own_admin))
-      (Mod.to_mod mod_tgt target_resource).
+    ∃ target_resource, refines_lmod
+      (Mod.to_lmod mod_top (IRΣ ⋅ ir_own_admin))
+      (Mod.to_lmod mod_tgt target_resource).
   Proof.
     move: (cancel_tgt)=>H; rewrite /refines in H; ss.
     hexploit H.
@@ -140,20 +157,19 @@ Module ClientAll.
     destruct (H (IRΣ ⋅ ir_own_admin)).
     { apply IRΣ_valid. }
     { clear H. simplify_res.
-      { iAssert (SchAS.tid_admin None) with "[H22]" as "TID".
+      { rewrite make_own_admin.
+        iAssert (winv (⊤, ⊤)) with "[H1 U W]" as "W".
+        { rewrite /winv; iFrame. }
+        iPoseProof (winv_split_empty with "W") as "[W $]".
+        iAssert (SchAS.tid_admin None) with "[H22]" as "TID".
         { rewrite /SchAS.tid_admin. unseal "SchA". eauto. }
-        iPoseProof (SchAS.tid_admin_none_split 0 with "TID") as "[TA TU]".
-        iSplitR "H1 TU U W".
-        - rewrite /init_cond. iSplitL "H24".
-          { iAssert (mem_init csl genv) with "[H24]" as "[$ _]". eauto. }
-          iSplitL "H8".
-          { rewrite /SchAS.init_threads. unseal "SchA". eauto. }
-          eauto.
-        - iPoseProof (make_own_admin with "H1") as "$".
-          unfold_pre_post; iFrame. done.
+        iMod (SchAS.tid_admin_none_split 0 with "TID") as "[TA TU]".
+        iSplitR "TU W H8 TA".
+        - rewrite /init_cond. iAssert (mem_init csl genv) with "[H24]" as "[$ _]". eauto. done.
+        - unfold_pre_post; iFrame. done.
       }
       all: solve_res.
     }
     { exists x; des; eauto. }
   (*SLOW*)Admitted.
-End ClientAll. *)
+End ClientAll.
